up to evalProgram made

TEEE.v
@@ -6,15 +6,8 @@ Inductive Types :=
  | function
  | millimeters
  | boolstate
- . 
+ .
  
-Inductive VarIdentifier :=
- | vnat : nat -> VarIdentifier
- | vReturn. 
- 
-Inductive TypedVar : Types -> Set  :=
- | VarRPMs : VarIdentifier -> nat -> TypedVar rpms.  
-
 
 Inductive Measurement : Type := 
  | MotorSpeed
@@ -59,27 +52,147 @@ Admitted.
 
 Definition Time := nat. 
 (* The calculation language *)
+(*  gives me trouble later when trying to create inductive eval. 
+Inductive Result (t : Types)  : Set:=
+ | result : (TypesDenote t) -> Result t.
+
+*)
+
+Inductive Result : Set :=
+ | result {t} : (TypesDenote t) -> Result. 
+
+
+  (*
+Definition resType ( r : Result) : Types :=
+match r with
+ | result t x => t
+end.
+
+Theorem resTypeIsCorrect : forall (r : Result), forall t, forall x, 
+  r = (result t x) -> resType r = t. 
+Proof. intros. rewrite H. simpl. reflexivity. 
+Qed.
+*)
+
+
+
 Inductive Calculation :=
- | calcValue (m : Measurement) : TypesDenote (measurementTypes m) -> Calculation
  | calcMeasure : Measurement -> Calculation 
- | calcAdd : Calculation -> Calculation.
+ | calcAdd : Calculation -> Calculation -> Calculation.
+ 
+Inductive TypedCalculation : Calculation -> Types ->  Prop := 
+ | TcalcMeasure : forall m, TypedCalculation (calcMeasure m) (measurementTypes m)
+ | TcalcAdd     : forall c1 c2 t1 t2, 
+     TypedCalculation c1 t1 -> 
+     TypedCalculation c2 t2 -> t1 = t2 -> TypedCalculation (calcAdd c1 c2) t1. 
 
-Definition add : Calcul
 
-Inductive EvalCalculation : Calculation -> Prop :=
- | evalcMeasure (m : Measurement) : EvalCalculation (calcMeasure m) ->
-     EvalCalculation (calcValue m (measure m)). 
- | evalcAdd (c1 c2 : Calculation, : Calculation -> EvalCalculation  Calculation. 
+Definition typeOf (r : Result) := 
+match r with
+ | @result t x => t
+end.
+Check typeOf.  
+
+(* dep typed version *)
+(*
+Definition addResults {t1 t2} (r1 r2 : (Result t)) (p : r1 = r2) : Result t.
+destruct t; (destruct r1 as [t1]); (destruct r2 as [t2]); simpl in t1; simpl in t2.
+exact (result rpms (t1 + t2)).
+exact (result meterscubedpersecond (t1 + t2)).
+exact (result volts (t1 + t2)).
+exact (result degreesC (t1 + t2)).
+exact (result function (fun x => t1 (t2 x))).
+exact (result millimeters (t1 + t2)).
+exact (result boolstate (andb t1 t2)).
+Defined.
+*)
+Definition addResult (r1 r2 : Result) {p : ((typeOf r1) = (typeOf r2))} : Result :=
+ match (r1,r2) with 
+  | (result v1, result v2) => r1
+ end. 
+ 
+ (* don't need. hopefully. *)
+ (*
+Inductive WResult : Set :=
+ | wr {t} : Result t -> WResult.
+
+Check @wr. 
+
+Definition resT {t} (x : (Result t)) := t.
+Definition getT (r : WResult) := 
+match r with
+ | wr x => (resT x)
+end.
+
+Definition unwrap (x : WResult) : (Result (getT x)).
+destruct x. simpl. exact r.
+Defined.
+
+Check unwrap.
+*)
+Inductive EvalCalculation : Calculation -> Result -> Prop :=
+ | evalcMeasure (m : Measurement) : EvalCalculation (calcMeasure m) 
+      (@result (measurementTypes m) (measure m))
+ | evalcAdd_same :
+      forall c1 c2 : Calculation, forall r1 r2, 
+      EvalCalculation c1 r1 ->
+      EvalCalculation c2 r2 ->
+      forall p : ((typeOf r1) = (typeOf r2)),
+      EvalCalculation (calcAdd c1 c2) ( (@addResult r1 r2 p)). 
+
+Inductive VarID :=
+ | vnat : nat -> VarID
+ | vReturn. 
+Require Import Coq.Classes.EquivDec.
+Theorem eq_dec_VarId : forall x y : VarID, {x = y} + {x <> y}.
+Proof. repeat decide equality. 
+Defined.
+  
+Inductive TypedVar : Types -> Set  :=
+ | VarRPMs : VarID -> nat -> TypedVar rpms.  
+
+
 Inductive Var :=
  | var : forall t : Types,  TypedVar t -> Var. 
 
 Inductive Program :=
- | Calc : Var ->  Calculation -> Program
- | Measure (m : Measurement) :
-     TypedVar (measurementTypes m) -> Program
+ | Calc : Types -> VarID ->  Calculation -> Program 
  | Delay : nat -> Program
- | Chain : Program -> Program -> Program.
+ | Chain : Program -> Program -> Program
+ | End.
+
+
+Definition VarState := list (VarID*Result).
  
-Inductive evalProgram :=
- | eCalc
- 
+Fixpoint lookup (vid : VarID) (vs : VarState) : option Result :=
+ match vs with 
+  | nil => None
+  | cons (vid',r) vs' => if  eq_dec_VarId vid vid' then Some r else 
+      lookup vid vs'
+ end. 
+
+
+Inductive State :=
+ | state : Time -> VarState -> State.
+Definition getVS (s : State) : VarState :=
+match s with
+ | state t vs => vs
+end. 
+
+Definition gettime (s : State) : Time :=
+match s with
+ | state t vs => t
+end.
+
+Inductive evalProgram : (Program * State) -> State -> Prop:=
+ | eCalc : forall c r id s, 
+             EvalCalculation c r -> evalProgram ((Calc (typeOf r) id c),s)
+                                      (state (gettime s) (cons (id,r) (getVS s))) 
+ | eDelay : forall n s, evalProgram ((Delay n),s) (state ((gettime s) + n) (getVS s))
+ | eChain : forall p1 p2 s1 s1' s2', 
+     evalProgram (p1,s1) s1' ->
+     evalProgram (p2, s1') s2' -> 
+     evalProgram (Chain p1 p2, s1) s2'. 
+
+
+ . 
